lib/FStar.TwoLevelHeap.fst
@@ -23,39 +23,37 @@ open FStar.Heap
 type rid = int  //region id
 type t = Map.t rid heap
 
-kind STPre = STPre_h t
-kind STPost (a:Type) = STPost_h t a
-kind STWP (a:Type) = STWP_h t a
+let st_pre = st_pre_h t
+let st_post (a:Type) = st_post_h t a
+let st_wp (a:Type) = st_wp_h t a
 new_effect STATE = STATE_h t
-effect State (a:Type) (wp:STWP a) =
+effect State (a:Type) (wp:st_wp a) =
        STATE a wp wp
-effect ST (a:Type) (pre:STPre) (post: (t -> STPost a)) =
+effect ST (a:Type) (pre:st_pre) (post: (t -> Tot (st_post a))) =
        STATE a
-             (fun (p:STPost a) (h:t) -> pre h /\ (forall a h1. post h a h1 ==> p a h1)) (* WP *)
-             (fun (p:STPost a) (h:t) -> (forall a h1. (pre h /\ post h a h1) ==> p a h1))          (* WLP *)
+             (fun (p:st_post a) (h:t) -> pre h /\ (forall a h1. post h a h1 ==> p a h1)) (* WP *)
+             (fun (p:st_post a) (h:t) -> (forall a h1. (pre h /\ post h a h1) ==> p a h1))          (* WLP *)
 effect St (a:Type) =
        ST a (fun h -> True) (fun h0 r h1 -> True)
 sub_effect
-  DIV   ~> STATE = fun (a:Type) (wp:PureWP a) (p:STPost a) (h:t) -> wp (fun a -> p a h)
+  DIV   ~> STATE = fun (a:Type) (wp:pure_wp a) (p:st_post a) (h:t) -> wp (fun a -> p a h)
 
 private type rref (id:rid) (a:Type) = ref a
 val as_ref : #a:Type -> #id:rid -> r:rref id a -> Tot (ref a)
-let as_ref id r = r
+let as_ref #a #id r = r
 
 private val ref_as_rref : #a:Type -> i:rid -> r:ref a -> Tot (rref i a)
-let ref_as_rref i r = r
+let ref_as_rref #a i r = r
 
 val lemma_as_ref_inj: #a:Type -> #i:rid -> r:rref i a
     -> Lemma (requires (True))
              (ensures ((ref_as_rref i (as_ref r) = r)))
        [SMTPat (as_ref r)]
-let lemma_as_ref_inj i r = ()
+let lemma_as_ref_inj #a #i r = ()
 
 assume val new_region: unit -> ST rid
       (requires (fun m -> True))
       (ensures (fun (m0:t) (id:rid) (m1:t) -> exists (h:heap). not(Map.contains m0 id) /\ m1=Map.upd m0 id h))
-
-type Let (#a:Type) (x:a) (body:(a -> Type)) = body x
 
 let sel (#a:Type) (#i:rid) (m:t) (r:rref i a) = Heap.sel (Map.sel m i) (as_ref r)
 let upd (#a:Type) (#i:rid) (m:t) (r:rref i a) (v:a) = Map.upd m i (Heap.upd (Map.sel m i) (as_ref r) v)
@@ -63,8 +61,8 @@ let upd (#a:Type) (#i:rid) (m:t) (r:rref i a) (v:a) = Map.upd m i (Heap.upd (Map
 assume val ralloc: #a:Type -> i:rid -> init:a -> ST (rref i a)
     (requires (fun m -> Map.contains m i))
     (ensures (fun m0 x m1 ->
-                    Let (Map.sel m0 i) (fun region_i ->
-                    not (Heap.contains region_i (as_ref x))
+                    let region_i = Map.sel m0 i in
+                    (not (Heap.contains region_i (as_ref x))
                     /\ m1=Map.upd m0 i (Heap.upd region_i (as_ref x) init))))
 
 assume val op_Colon_Equals: #a:Type -> #i:rid -> r:rref i a -> v:a -> ST unit
@@ -79,16 +77,16 @@ assume val get: unit -> ST t
   (requires (fun m -> True))
   (ensures (fun m0 x m1 -> m0=x /\ m1=m0))
 
-type modifies (s:Set.set rid) (m0:t) (m1:t) =
+let modifies (s:Set.set rid) (m0:t) (m1:t) =
     Map.Equal m1 (Map.concat m1 (Map.restrict (Set.complement s) m0))
 
-type fresh_region (i:rid) (m0:t) (m1:t) =
+let fresh_region (i:rid) (m0:t) (m1:t) =
   not (Map.contains m0 i)
   /\ Map.contains m1 i
 
-type contains_ref (#a:Type) (#i:rid) (r:rref i a) (m:t) =
+let contains_ref (#a:Type) (#i:rid) (r:rref i a) (m:t) =
     Map.contains m i /\ Heap.contains (Map.sel m i) (as_ref r)
 
-type fresh_rref (#a:Type) (#i:rid) (r:rref i a) (m0:t) (m1:t) =
+let fresh_rref (#a:Type) (#i:rid) (r:rref i a) (m0:t) (m1:t) =
   not (Heap.contains (Map.sel m0 i) (as_ref r))
   /\  (Heap.contains (Map.sel m1 i) (as_ref r))
